Add reserve

src/model/Cell.v
@@ -1,5 +1,7 @@
 Require Import RelationClasses.
 Require Import ZArith.
+Require Import Decidable.
+Require Import Coq.Lists.ListDec.
 
 From sflib Require Import sflib.
 
@@ -17,46 +19,49 @@ Set Implicit Arguments.
 
 
 Module Message.
-  Variant t := mk (val: Const.t) (released: option View.t) (na: bool).
+  Variant t :=
+    | message (val: Const.t) (released: option View.t) (na: bool)
+    | reserve
+  .
 
-  Definition elt: t := mk 0%Z None true.
+  Definition elt: t := message 0%Z None true.
 
   Variant wf: t -> Prop :=
-  | wf_intro
-      val released na
-      (RELEASED: View.opt_wf released):
-    wf (mk val released na)
+    | wf_message
+        val released na
+        (RELEASED: View.opt_wf released):
+      wf (message val released na)
+    | wf_reserve:
+      wf reserve
   .
   #[global] Hint Constructors wf: core.
 
   Definition elt_wf: wf elt.
-  Proof. ss. Qed.
+  Proof.
+    econs. ss.
+  Qed.
 
   Variant le: t -> t -> Prop :=
-  | le_intro
-      val1 released1 na1
-      val2 released2 na2
-      (VAL: Const.le val2 val1)
-      (RELEASED: View.opt_le released1 released2)
-      (NA: implb na2 na1):
-    le (mk val1 released1 na1) (mk val2 released2 na2)
+    | le_message
+        val1 released1 na1
+        val2 released2 na2
+        (VAL: Const.le val2 val1)
+        (RELEASED: View.opt_le released1 released2)
+        (NA: implb na2 na1):
+      le (message val1 released1 na1) (message val2 released2 na2)
+    | le_reserve:
+      le reserve reserve
   .
   #[global] Hint Constructors le: core.
 
   Global Program Instance le_PreOrder: PreOrder le.
   Next Obligation.
-    ii. destruct x. econs; try refl. destruct na; ss.
+    ii. destruct x; ss. econs; try refl. destruct na; ss.
   Qed.
   Next Obligation.
-    ii. inv H. inv H0. econs; try by (etrans; eauto).
+    ii. inv H; inv H0; ss. econs; try by (etrans; eauto).
     destruct na1, na2, na3; ss.
   Qed.
-
-  Definition is_released_none (msg: t): bool :=
-    match msg with
-    | mk _ None _ => true
-    | _ => false
-    end.
 End Message.
 #[export] Hint Constructors Message.wf: core.
 
@@ -179,6 +184,43 @@ Module Cell.
         + inv GET2. inv ADD. symmetry. hexploit DISJOINT0; eauto.
         + eapply DISJOINT; eauto.
     Qed.
+
+    Inductive remove (cell1:t) (from to:Time.t) (msg:Message.t) (cell2:t): Prop :=
+    | remove_intro
+        (GET: DOMap.find to cell1 = Some (from, msg))
+        (CELL2: cell2 = DOMap.remove to cell1)
+    .
+    #[global] Hint Constructors remove: core.
+
+    Lemma remove_o
+          cell2 cell1 from to msg
+          t
+          (REMOVE: remove cell1 from to msg cell2):
+      DOMap.find t cell2 =
+      if Time.eq_dec t to
+      then None
+      else DOMap.find t cell1.
+    Proof.
+      inv REMOVE. rewrite DOMap.grspec.
+      repeat condtac; auto; congr.
+    Qed.
+
+    Lemma remove_wf
+          cell1 from to msg cell2
+          (REMOVE: remove cell1 from to msg cell2)
+          (CELL1: wf cell1):
+      wf cell2.
+    Proof.
+      inv CELL1. econs; i.
+      - revert GET. erewrite remove_o; eauto. condtac; try congr.
+        i. eapply VOLUME; eauto.
+      - revert GET. erewrite remove_o; eauto. condtac; ss. apply WF.
+      - revert GET1 GET2.
+        erewrite (remove_o to1); eauto.
+        erewrite (remove_o to2); eauto.
+        repeat condtac; repeat subst; try congr; i.
+        eapply DISJOINT; eauto.
+    Qed.
   End Raw.
 
   Structure t := mk {
@@ -186,7 +228,8 @@ Module Cell.
     WF: Raw.wf raw;
   }.
 
-  Definition get (ts:Time.t) (cell:t): option (Time.t * Message.t) := DOMap.find ts (raw cell).
+  Definition get (ts:Time.t) (cell:t): option (Time.t * Message.t) :=
+    DOMap.find ts (raw cell).
 
   Lemma ext
         (lhs rhs:t)
@@ -287,15 +330,8 @@ Module Cell.
   Definition add (cell1:t) (from to:Time.t) (msg: Message.t) (cell2:t): Prop :=
     Raw.add cell1 from to msg cell2.
 
-  Lemma add_o
-        cell2 cell1 from to msg
-        t
-        (ADD: add cell1 from to msg cell2):
-    get t cell2 =
-    if Time.eq_dec t to
-    then Some (from, msg)
-    else get t cell1.
-  Proof. apply Raw.add_o. auto. Qed.
+  Definition remove (cell1:t) (from to:Time.t) (msg: Message.t) (cell2:t): Prop :=
+    Raw.remove cell1 from to msg cell2.
 
   Definition max_ts (cell:t): Time.t :=
     DOMap.max_key (raw cell).
@@ -315,6 +351,19 @@ Module Cell.
       + exfalso. eapply FIND; eauto. rewrite GET. congr.
     - apply MAX. rewrite GET. auto. congr.
   Qed.
+
+
+  (* Lemmas on add *)
+
+  Lemma add_o
+        cell2 cell1 from to msg
+        t
+        (ADD: add cell1 from to msg cell2):
+    get t cell2 =
+    if Time.eq_dec t to
+    then Some (from, msg)
+    else get t cell1.
+  Proof. apply Raw.add_o. auto. Qed.
 
   Lemma add_exists
         cell1 from to msg
@@ -351,9 +400,6 @@ Module Cell.
     inv ADD. apply add_exists; auto. i.
     eapply DISJOINT. eauto.
   Qed.
-
-
-  (* Lemmas on add *)
 
   Lemma add_get0
         cell1 from1 to1 msg1 cell2
@@ -408,12 +454,40 @@ Module Cell.
     - eapply max_ts_spec. erewrite add_o; eauto. condtac; ss.
   Qed.
 
-  Lemma get_opt_wf
-        cell from to msg
-        (GET: get to cell = Some (from, msg)):
-    Message.wf msg.
+
+  (* lemmas on remove *)
+
+  Lemma remove_o
+        cell2 cell1 from to msg
+        t
+        (REMOVE: remove cell1 from to msg cell2):
+    get t cell2 =
+    if Time.eq_dec t to
+    then None
+    else get t cell1.
+  Proof. eapply Raw.remove_o. eauto. Qed.
+
+  Lemma remove_exists
+        cell1 from to msg
+        (GET: get to cell1 = Some (from, msg)):
+    exists cell2, remove cell1 from to msg cell2.
   Proof.
-    destruct cell. destruct WF0. eauto.
+    eexists (mk _). destruct cell1. ss.
+    Unshelve.
+    { eapply Raw.remove_wf.
+      - econs; eauto.
+      - apply WF.
+    }
+  Qed.
+
+  Lemma remove_get0
+        cell1 from to msg cell2
+        (REMOVE: remove cell1 from to msg cell2):
+    <<GET: get to cell1 = Some (from, msg)>> /\
+    <<GET: get to cell2 = None>>.
+  Proof.
+    inv REMOVE. splits; auto.
+    unfold get. rewrite CELL2. rewrite DOMap.grspec. condtac; ss.
   Qed.
 
 
@@ -693,5 +767,277 @@ Module Cell.
     - exploit DOMap.elements_correct; try exact INHABITED. i.
       exploit in_prod; try exact x0. i.
       exploit prev_spec_None; eauto. i. timetac.
+  Qed.
+
+
+  (* adjacent *)
+
+  Inductive adjacent (from1 to1 from2 to2: Time.t) (cell: t): Prop :=
+  | adjacent_intro
+      m1 m2
+      (GET1: get to1 cell = Some (from1, m1))
+      (GET2: get to2 cell = Some (from2, m2))
+      (TS: Time.lt to1 to2)
+      (EMPTY: forall ts (TS1: Time.lt to1 ts) (TS2: Time.le ts from2),
+          get ts cell = None)
+  .
+
+  Lemma adjacent_ts
+        from1 to1 from2 to2 mem
+        (ADJ: adjacent from1 to1 from2 to2 mem):
+    Time.le to1 from2.
+  Proof.
+    destruct (Time.le_lt_dec to1 from2); auto.
+    exfalso. inv ADJ.
+    exploit get_ts; try exact GET1. i. des.
+    { subst. inv l. }
+    exploit get_ts; try exact GET2. i. des.
+    { subst. inv TS. }
+    exploit get_disjoint; [exact GET1|exact GET2|..]. i. des.
+    { subst. timetac. }
+    apply (x2 to1); econs; ss.
+    - refl.
+    - econs. auto.
+  Qed.
+
+  Lemma adjacent_inj
+        to mem
+        from1 from2 from3 to3 from4 to4
+        (ADJ1: adjacent from1 to from3 to3 mem)
+        (ADJ2: adjacent from2 to from4 to4 mem):
+    from1 = from2 /\ from3 = from4 /\ to3 = to4.
+  Proof.
+    inv ADJ1. inv ADJ2.
+    rewrite GET1 in GET0. inv GET0.
+    destruct (Time.le_lt_dec to3 to4); cycle 1.
+    { exfalso.
+      destruct (Time.le_lt_dec to4 from3).
+      - exploit EMPTY; try exact l0; eauto. i. congr.
+      - exploit get_ts; try exact GET2. i. des.
+        { subst. inv l. }
+        exploit get_ts; try exact GET3. i. des.
+        { subst. inv l0. }
+        exploit get_disjoint; [exact GET2|exact GET3|..]. i. des.
+        { subst. timetac. }
+        apply (x2 to4); econs; ss.
+        + econs. ss.
+        + refl. }
+    inv l.
+    { exfalso.
+      destruct (Time.le_lt_dec to3 from4).
+      - exploit EMPTY0; try exact l; eauto. i. congr.
+      - exploit get_ts; try exact GET2. i. des.
+        { subst. inv l. }
+        exploit get_ts; try exact GET3. i. des.
+        { subst. inv H. }
+        exploit get_disjoint; [exact GET2|exact GET3|..]. i. des.
+        { subst. timetac. }
+        apply (x2 to3); econs; ss.
+        + refl.
+        + econs. ss. }
+    inv H. rewrite GET2 in GET3. inv GET3.
+    splits; auto.
+  Qed.
+
+  Lemma adjacent_exists
+        from1 to1 msg cell
+        (GET: get to1 cell = Some (from1, msg))
+        (TO: Time.lt to1 (max_ts cell)):
+    exists from2 to2,
+      adjacent from1 to1 from2 to2 cell.
+  Proof.
+    exploit next_exists; eauto. i. des.
+    esplits. econs; try exact x0; eauto. i.
+    eapply x2; eauto.
+    exploit get_ts; try exact x0. i. des.
+    - subst. inv x1.
+    - eapply TimeFacts.le_lt_lt; eauto.
+  Qed.
+
+
+  (* cap *)
+
+  Inductive cap (cell1 cell2: t): Prop :=
+  | cap_intro
+      (SOUND: le cell1 cell2)
+      (MIDDLE: forall from1 to1 from2 to2
+                 (ADJ: adjacent from1 to1 from2 to2 cell1)
+                 (TO: Time.lt to1 from2),
+          get from2 cell2 = Some (to1, Message.reserve))
+      (BACK: get (Time.incr (max_ts cell1)) cell2 =
+             Some (max_ts cell1, Message.reserve))
+      (COMPLETE: forall from to msg
+                   (GET1: get to cell1 = None)
+                   (GET2: get to cell2 = Some (from, msg)),
+          (exists f m, get from cell1 = Some (f, m)))
+  .
+
+  Inductive cap_aux (dom: list Time.t) (cell1 cell2: t): Prop :=
+  | cap_aux_intro
+      (SOUND: le cell1 cell2)
+      (MIDDLE: forall from1 to1 from2 to2
+                 (IN: List.In to1 dom)
+                 (ADJ: adjacent from1 to1 from2 to2 cell1)
+                 (TO: Time.lt to1 from2),
+          get from2 cell2 = Some (to1, Message.reserve))
+      (BACK: forall (IN: List.In (max_ts cell1) dom),
+          get (Time.incr (max_ts cell1)) cell2 =
+          Some (max_ts cell1, Message.reserve))
+      (COMPLETE: forall from to msg
+                   (GET1: get to cell1 = None)
+                   (GET2: get to cell2 = Some (from, msg)),
+          List.In from dom /\
+          (exists f m, get from cell1 = Some (f, m)))
+  .
+
+  Lemma cap_aux_exists
+        dom cell1
+        (INHABITED: get Time.bot cell1 = Some (Time.bot, Message.elt)):
+    exists cell2, cap_aux dom cell1 cell2.
+  Proof.
+    revert cell1 INHABITED.
+    induction dom; i.
+    { exists cell1. econs; ss; i. congr. }
+    exploit IHdom; eauto. intros x. des. clear IHdom.
+    destruct (In_decidable time_decidable a dom).
+    { exists cell2. inv x. econs; ii; eauto.
+      - inv IN; eauto.
+      - inv IN; eauto.
+      - exploit COMPLETE; eauto. i. des.
+        split; eauto. econs 2; eauto.
+    }
+    destruct (get a cell1) as [[from msg]|] eqn:GET1; cycle 1.
+    { exists cell2. inv x. econs; ii; eauto.
+      - inv IN; eauto. inv ADJ. congr.
+      - inv IN; eauto.
+        exploit max_ts_spec; eauto. i. des. congr.
+      - exploit COMPLETE; eauto. i. des.
+        split; eauto. econs 2; eauto.
+    }
+    exploit max_ts_spec; eauto. i. des.
+    inv MAX.
+    { exploit adjacent_exists; try exact GET1; ss. i. des.
+      exploit adjacent_ts; eauto. i. inv x2; cycle 1.
+      { inv H1.
+        exists cell2. inv x. econs; ii; eauto.
+        - inv IN; eauto.
+          exploit adjacent_inj; [exact x1|exact ADJ|..]. i. des. subst.
+          timetac.
+        - inv IN; eauto. timetac.
+        - exploit COMPLETE; eauto. i. des.
+          split; eauto. econs 2; eauto.
+      }
+      exploit (@add_exists cell2 a from2 Message.reserve); ii.
+      { inv x. inv x1. inv LHS. inv RHS. ss.
+        clear MIDDLE BACK.
+        destruct (get to0 cell1) as [[]|] eqn:GET4.
+        - exploit SOUND; try exact GET4. intros x.
+          rewrite x in *. inv GET2.
+          destruct (Time.le_lt_dec to0 from2).
+          { exploit (EMPTY to0); try congr.
+            eapply TimeFacts.lt_le_lt; try exact FROM; ss. }
+          exploit get_ts; try exact GET3. i. des.
+          { subst. inv TS. }
+          exploit get_ts; try exact GET4. i. des.
+          { subst. inv l. }
+          exploit get_disjoint; [exact GET3|exact GET4|..]. i. des.
+          { subst. timetac. }
+          destruct (Time.le_lt_dec to0 to2).
+          + apply (x4 to0); econs; ss; try refl.
+          + apply (x4 to2); econs; ss; try refl.
+            * eapply TimeFacts.le_lt_lt; try exact x2.
+              etrans; try exact TO. econs. ss.
+            * econs. ss.
+        - exploit COMPLETE; try exact GET2; eauto. intros x. des.
+          cut (from1 = a); try by (i; subst; ss).
+          clear COMPLETE.
+          destruct (Time.le_lt_dec from1 a).
+          + inv l; try by (inv H2; ss).
+            exploit SOUND; try exact GET0. intros x2.
+            exploit get_ts; try exact x2. i. des.
+            { subst. inv H2. }
+            exploit get_disjoint; [exact x2|exact GET2|..]. i. des.
+            { subst. timetac. }
+            exfalso.
+            apply (x5 a); econs; ss; try refl.
+            econs. eapply TimeFacts.lt_le_lt; try exact FROM. ss.
+          + exploit (EMPTY from1); try congr.
+            econs. eapply TimeFacts.lt_le_lt; try exact FROM0. ss.
+      }
+      { ss. }
+      { econs. }
+      des.
+      exists cell0. inv x. econs; ii; ss.
+      - exploit SOUND; eauto. i.
+        eapply add_get1; eauto.
+      - exploit add_get0; eauto. i. des.
+        des; subst.
+        + exploit adjacent_inj; [exact x1|exact ADJ|..]. i. des.
+          subst. ss.
+        + exploit MIDDLE; eauto. i.
+          eapply add_get1; eauto.
+      - des; subst; timetac.
+        exploit BACK; eauto. i.
+        eapply add_get1; eauto.
+      - revert GET2. erewrite add_o; eauto. condtac; ss; i.
+        + subst. inv GET2. splits; eauto.
+        + exploit COMPLETE; eauto. i. des.
+          esplits; eauto.
+    }
+    inv H0. clear from0 msg0 GET.
+    exploit (@add_exists cell2 (max_ts cell1) (Time.incr (max_ts cell1)) Message.reserve); ii.
+    { inv x. inv LHS. inv RHS. ss.
+      destruct (get to2 cell1) as [[]|] eqn:GET3.
+      { exploit SOUND; eauto. intros x.
+        rewrite x in *. inv GET2.
+        exploit max_ts_spec; try exact GET3. i. des.
+        exploit TimeFacts.le_lt_lt; try exact FROM; try exact MAX. i.
+        timetac. }
+      exploit COMPLETE; eauto. intros x. des.
+      cut (from2 = max_ts cell1); try by (i; subst; ss).
+      destruct (Time.le_lt_dec from2 (max_ts cell1)).
+      - inv l; try by (inv H0; ss).
+        exploit SOUND; try exact GET1. intros x2.
+        exploit get_ts; try exact x2. i. des.
+        { subst. rewrite x3 in *. inv H0. }
+        exploit get_ts; try exact GET2. i. des.
+        { subst. timetac. }
+        exploit get_disjoint; [exact x2|exact GET2|..]. i. des.
+        { subst. timetac. }
+        exfalso.
+        apply (x6 (max_ts cell1)); econs; ss; try refl.
+        econs. eapply TimeFacts.lt_le_lt; try exact FROM. ss.
+      - exploit max_ts_spec; try exact x1. i. des.
+        timetac.
+    }
+    { apply Time.incr_spec. }
+    { econs. }
+    des.
+    exists cell0. inv x. econs; ii; ss; eauto.
+    - exploit SOUND; eauto. i.
+      eapply add_get1; eauto.
+    - exploit add_get0; eauto. i. des.
+      + inv ADJ. exploit max_ts_spec; try exact GET3. i. des. timetac.
+      + eapply add_get1; eauto.
+    - eapply add_get0; eauto.
+    - revert GET2. erewrite add_o; eauto. condtac; ss; i.
+      + subst. inv GET2. esplits; eauto.
+      + exploit COMPLETE; eauto. i. des.
+        esplits; eauto.
+  Qed.
+
+  Lemma cap_exists
+        cell1
+        (INHABITED: get Time.bot cell1 = Some (Time.bot, Message.elt)):
+    exists cell2, cap cell1 cell2.
+  Proof.
+    destruct (@finite cell1).
+    exploit (@cap_aux_exists x); eauto. i. des.
+    exists cell2. inv x1. econs; i; ss; eauto.
+    - eapply MIDDLE; eauto. inv ADJ. eauto.
+    - eapply BACK; eauto.
+      exploit max_ts_spec; eauto. i. des. eauto.
+    - exploit COMPLETE; eauto. i. des.
+      esplits; eauto.
   Qed.
 End Cell.
